formalization/Push_Relabel_Maxflow/Prpu_Benchmark_Export.thy
@@ -27,7 +27,8 @@ code_printing
   (**)
   export_code nat_of_integer integer_of_nat int_of_integer integer_of_int
   prepareNet 
-  (*relabel_to_front_impl*) relabel_to_front_impl_tab_am fifo_push_relabel
+  relabel_to_front_impl relabel_to_front_impl_tab_am 
+  fifo_push_relabel fifo_push_relabel_prepare_impl fifo_push_relabel_run_impl
   in SML_imp 
   module_name Prpu
   file "evaluation/prpu-SML/Prpu_Export.sml"  
