formalization/Push_Relabel_Maxflow/evaluation/bench_exec.sh
@@ -1,8 +1,34 @@
 #!/bin/bash
 
-tests=`cat tests`
-platforms_fofu=`cat fofu-platforms`
-platforms_prpu=`cat prpu-platforms`
+for i in "$@"
+do
+case $i in
+    --tests=*)
+    tests="${i#*=}"
+    shift
+    ;;
+    --fofu=*)
+    platforms_fofu="${i#*=}"
+    shift
+    ;;
+    --prpu=*)
+    platforms_prpu="${i#*=}"
+    shift
+    ;;
+    *)
+      echo "Unknown command line argument: $i"
+      exit 1
+    ;;
+esac
+done
+
+
+test -n "$tests" || tests=`cat tests`
+test -n "$platforms_fofu" || platforms_fofu=`cat fofu-platforms`
+test -n "$platforms_prpu" || platforms_prpu=`cat prpu-platforms`
+
+test "$platforms_fofu" = "-" &&  platforms_fofu=""
+test "$platforms_prpu" = "-" &&  platforms_prpu=""
 
 for t in $tests; do
   echo "*********************"
